theories/Numbers/Integer/BigZ/BigZ.v
@@ -11,50 +11,99 @@
 (*i $Id$ i*)
 
 Require Export BigN.
+Require Import ZTimesOrder.
+Require Import ZSig.
+Require Import ZSigZAxioms.
 Require Import ZMake.
 
+Module BigZ <: ZType := ZMake.Make BigN.
 
-Module BigZ := Make BigN.
+(** Module [BigZ] implements [ZAxiomsSig] *)
 
+Module Export BigZAxiomsMod := ZSig_ZAxioms BigZ.
+Module Export BigZTimesOrderPropMod := ZTimesOrderPropFunct BigZAxiomsMod.
 
-Definition bigZ := BigZ.t.
+(** Notations about [BigZ] *)
+
+Notation bigZ := BigZ.t.
 
 Delimit Scope bigZ_scope with bigZ.
 Bind Scope bigZ_scope with bigZ.
 Bind Scope bigZ_scope with BigZ.t.
 Bind Scope bigZ_scope with BigZ.t_.
 
-Notation " i + j " := (BigZ.add i j) : bigZ_scope.
-Notation " i - j " := (BigZ.sub i j) : bigZ_scope.
-Notation " i * j " := (BigZ.mul i j) : bigZ_scope.
-Notation " i / j " := (BigZ.div i j) : bigZ_scope.
-Notation " i ?= j " := (BigZ.compare i j) : bigZ_scope.
+Notation Local "0" := BigZ.zero : bigZ_scope.
+Infix "+" := BigZ.add : bigZ_scope.
+Infix "-" := BigZ.sub : bigZ_scope.
+Notation "- x" := (BigZ.opp x) : bigZ_scope.
+Infix "*" := BigZ.mul : bigZ_scope.
+Infix "/" := BigZ.div : bigZ_scope.
+Infix "?=" := BigZ.compare : bigZ_scope.
+Infix "==" := BigZ.eq (at level 70, no associativity) : bigZ_scope.
+Infix "<" := BigZ.lt : bigZ_scope.
+Infix "<=" := BigZ.le : bigZ_scope.
+Notation "[ i ]" := (BigZ.to_Z i) : bigZ_scope.
 
+Open Scope bigZ_scope.
 
- Theorem spec_to_Z: 
-  forall n, BigN.to_Z (BigZ.to_N n) = 
-            (Zsgn (BigZ.to_Z n) * BigZ.to_Z n)%Z.
- intros n; case n; simpl; intros p; 
-     generalize (BigN.spec_pos p); case (BigN.to_Z p); auto.
- intros p1 H1; case H1; auto.
- intros p1 H1; case H1; auto.
- Qed.
+(** Some additional results about [BigZ] *)
 
- Theorem spec_to_N n: 
-  (BigZ.to_Z n = 
-    Zsgn (BigZ.to_Z n) * (BigN.to_Z (BigZ.to_N n)))%Z.
- intros n; case n; simpl; intros p; 
-     generalize (BigN.spec_pos p); case (BigN.to_Z p); auto.
- intros p1 H1; case H1; auto.
- intros p1 H1; case H1; auto.
- Qed.
+Theorem spec_to_Z: forall n:bigZ, 
+  BigN.to_Z (BigZ.to_N n) = ((Zsgn [n]) * [n])%Z.
+Proof.
+intros n; case n; simpl; intros p; 
+  generalize (BigN.spec_pos p); case (BigN.to_Z p); auto.
+intros p1 H1; case H1; auto.
+intros p1 H1; case H1; auto.
+Qed.
 
- Theorem spec_to_Z_pos: 
-  forall n, (0 <= BigZ.to_Z n ->
-              BigN.to_Z (BigZ.to_N n) = BigZ.to_Z n)%Z.
- intros n; case n; simpl; intros p; 
-     generalize (BigN.spec_pos p); case (BigN.to_Z p); auto.
- intros p1 _  H1; case H1; auto.
- intros p1 H1; case H1; auto.
- Qed.
+Theorem spec_to_N n: 
+ ([n] = Zsgn [n] * (BigN.to_Z (BigZ.to_N n)))%Z.
+Proof.
+intros n; case n; simpl; intros p; 
+  generalize (BigN.spec_pos p); case (BigN.to_Z p); auto.
+intros p1 H1; case H1; auto.
+intros p1 H1; case H1; auto.
+Qed.
 
+Theorem spec_to_Z_pos: forall n, (0 <= [n])%Z ->
+  BigN.to_Z (BigZ.to_N n) = [n].
+Proof.
+intros n; case n; simpl; intros p; 
+  generalize (BigN.spec_pos p); case (BigN.to_Z p); auto.
+intros p1 _ H1; case H1; auto.
+intros p1 H1; case H1; auto.
+Qed.
+
+Lemma sub_opp : forall x y : bigZ, x - y == x + (- y).
+Proof.
+red; intros; zsimpl; auto.
+Qed.
+
+Lemma plus_opp : forall x : bigZ, x + (- x) == 0.
+Proof.
+red; intros; zsimpl; auto with zarith.
+Qed.
+
+(** [BigZ] is a ring *)
+
+Lemma BigZring : 
+ ring_theory BigZ.zero BigZ.one BigZ.add BigZ.mul BigZ.sub BigZ.opp BigZ.eq.
+Proof.
+constructor.
+exact Zplus_0_l.
+exact Zplus_comm.
+exact Zplus_assoc.
+exact Ztimes_1_l.
+exact Ztimes_comm.
+exact Ztimes_assoc.
+exact Ztimes_plus_distr_r.
+exact sub_opp.
+exact plus_opp.
+Qed.
+
+Add Ring BigZr : BigZring.
+
+(** Todo: tactic translating from [BigZ] to [Z] + omega *)
+
+(** Todo: micromega *)
