theories/Numbers/Integer/SpecViaZ/ZSigZAxioms.v
@@ -1,0 +1,306 @@
+(************************************************************************)
+(*  v      *   The Coq Proof Assistant  /  The Coq Development Team     *)
+(* <O___,, * CNRS-Ecole Polytechnique-INRIA Futurs-Universite Paris Sud *)
+(*   \VV/  **************************************************************)
+(*    //   *      This file is distributed under the terms of the       *)
+(*         *       GNU Lesser General Public License Version 2.1        *)
+(************************************************************************)
+
+(*i $Id$ i*)
+
+Require Import ZArith.
+Require Import ZAxioms.
+Require Import ZSig.
+
+(** * The interface [ZSig.ZType] implies the interface [ZAxiomsSig] *)
+
+Module ZSig_ZAxioms (Z:ZType) <: ZAxiomsSig.
+
+Delimit Scope IntScope with Int.
+Bind Scope IntScope with Z.t.
+Open Local Scope IntScope.
+Notation "[ x ]" := (Z.to_Z x) : IntScope.
+Infix "=="  := Z.eq (at level 70) : IntScope.
+Notation "0" := Z.zero : IntScope.
+Infix "+" := Z.add : IntScope.
+Infix "-" := Z.sub : IntScope.
+Infix "*" := Z.mul : IntScope.
+Notation "- x" := (Z.opp x) : IntScope.
+
+Hint Rewrite 
+ Z.spec_0 Z.spec_1 Z.spec_add Z.spec_sub Z.spec_pred Z.spec_succ
+ Z.spec_mul Z.spec_opp Z.spec_of_Z : Zspec.
+
+Ltac zsimpl := unfold Z.eq in *; autorewrite with Zspec.
+
+Module Export NZOrdAxiomsMod <: NZOrdAxiomsSig.
+Module Export NZAxiomsMod <: NZAxiomsSig.
+
+Definition NZ := Z.t.
+Definition NZeq := Z.eq.
+Definition NZ0 := Z.zero.
+Definition NZsucc := Z.succ.
+Definition NZpred := Z.pred.
+Definition NZplus := Z.add.
+Definition NZminus := Z.sub.
+Definition NZtimes := Z.mul.
+
+Theorem NZeq_equiv : equiv Z.t Z.eq.
+Proof.
+repeat split; repeat red; intros; auto; congruence.
+Qed.
+
+Add Relation Z.t Z.eq
+ reflexivity proved by (proj1 NZeq_equiv)
+ symmetry proved by (proj2 (proj2 NZeq_equiv))
+ transitivity proved by (proj1 (proj2 NZeq_equiv))
+ as NZeq_rel.
+
+Add Morphism NZsucc with signature Z.eq ==> Z.eq as NZsucc_wd.
+Proof.
+intros; zsimpl; f_equal; assumption.
+Qed.
+
+Add Morphism NZpred with signature Z.eq ==> Z.eq as NZpred_wd.
+Proof.
+intros; zsimpl; f_equal; assumption.
+Qed.
+
+Add Morphism NZplus with signature Z.eq ==> Z.eq ==> Z.eq as NZplus_wd.
+Proof.
+intros; zsimpl; f_equal; assumption.
+Qed.
+
+Add Morphism NZminus with signature Z.eq ==> Z.eq ==> Z.eq as NZminus_wd.
+Proof.
+intros; zsimpl; f_equal; assumption.
+Qed.
+
+Add Morphism NZtimes with signature Z.eq ==> Z.eq ==> Z.eq as NZtimes_wd.
+Proof.
+intros; zsimpl; f_equal; assumption.
+Qed.
+
+Theorem NZpred_succ : forall n, Z.pred (Z.succ n) == n.
+Proof.
+intros; zsimpl; auto with zarith.
+Qed.
+
+Section Induction.
+
+Variable A : Z.t -> Prop.
+Hypothesis A_wd : predicate_wd Z.eq A.
+Hypothesis A0 : A 0.
+Hypothesis AS : forall n, A n <-> A (Z.succ n). 
+
+Add Morphism A with signature Z.eq ==> iff as A_morph.
+Proof. apply A_wd. Qed.
+
+Let B (z : Z) := A (Z.of_Z z).
+
+Lemma B0 : B 0.
+Proof.
+unfold B; simpl.
+rewrite <- (A_wd 0); auto.
+zsimpl; auto.
+Qed.
+
+Lemma BS : forall z : Z, B z -> B (z + 1).
+Proof.
+intros z H.
+unfold B in *. apply -> AS in H.
+setoid_replace (Z.of_Z (z + 1)) with (Z.succ (Z.of_Z z)); auto.
+zsimpl; auto.
+Qed.
+
+Lemma BP : forall z : Z, B z -> B (z - 1).
+Proof.
+intros z H.
+unfold B in *. rewrite AS.
+setoid_replace (Z.succ (Z.of_Z (z - 1))) with (Z.of_Z z); auto.
+zsimpl; auto with zarith.
+Qed.
+
+Lemma B_holds : forall z : Z, B z.
+Proof.
+intros; destruct (Z_lt_le_dec 0 z).
+apply natlike_ind; auto with zarith.
+apply B0.
+intros; apply BS; auto.
+replace z with (-(-z))%Z in * by (auto with zarith).
+remember (-z)%Z as z'.
+pattern z'; apply natlike_ind.
+apply B0.
+intros; rewrite Zopp_succ; unfold Zpred; apply BP; auto.
+subst z'; auto with zarith.
+Qed.
+
+Theorem NZinduction : forall n, A n.
+Proof.
+intro n. setoid_replace n with (Z.of_Z (Z.to_Z n)).
+apply B_holds.
+zsimpl; auto.
+Qed.
+
+End Induction.
+
+Theorem NZplus_0_l : forall n, 0 + n == n.
+Proof.
+intros; zsimpl; auto with zarith.
+Qed.
+
+Theorem NZplus_succ_l : forall n m, (Z.succ n) + m == Z.succ (n + m).
+Proof.
+intros; zsimpl; auto with zarith.
+Qed.
+
+Theorem NZminus_0_r : forall n, n - 0 == n.
+Proof.
+intros; zsimpl; auto with zarith.
+Qed.
+
+Theorem NZminus_succ_r : forall n m, n - (Z.succ m) == Z.pred (n - m).
+Proof.
+intros; zsimpl; auto with zarith.
+Qed.
+
+Theorem NZtimes_0_l : forall n, 0 * n == 0.
+Proof.
+intros; zsimpl; auto with zarith.
+Qed.
+
+Theorem NZtimes_succ_l : forall n m, (Z.succ n) * m == n * m + m.
+Proof.
+intros; zsimpl; ring.
+Qed.
+
+End NZAxiomsMod.
+
+Definition NZlt := Z.lt.
+Definition NZle := Z.le.
+Definition NZmin := Z.min.
+Definition NZmax := Z.max.
+
+Infix "<=" := Z.le : IntScope.
+Infix "<" := Z.lt : IntScope.
+
+Lemma spec_compare_alt : forall x y, Z.compare x y = ([x] ?= [y])%Z.
+Proof.
+ intros; generalize (Z.spec_compare x y).
+ destruct (Z.compare x y); auto.
+ intros H; rewrite H; symmetry; apply Zcompare_refl.
+Qed.
+
+Lemma spec_lt : forall x y, (x<y) <-> ([x]<[y])%Z.
+Proof.
+ intros; unfold Z.lt, Zlt; rewrite spec_compare_alt; intuition.
+Qed.
+
+Lemma spec_le : forall x y, (x<=y) <-> ([x]<=[y])%Z.
+Proof.
+ intros; unfold Z.le, Zle; rewrite spec_compare_alt; intuition.
+Qed.
+
+Lemma spec_min : forall x y, [Z.min x y] = Zmin [x] [y].
+Proof.
+ intros; unfold Z.min, Zmin.
+ rewrite spec_compare_alt; destruct Zcompare; auto.
+Qed.
+
+Lemma spec_max : forall x y, [Z.max x y] = Zmax [x] [y].
+Proof.
+ intros; unfold Z.max, Zmax.
+ rewrite spec_compare_alt; destruct Zcompare; auto.
+Qed.
+
+Add Morphism Z.compare with signature Z.eq ==> Z.eq ==> (@eq comparison) as compare_wd.
+Proof. 
+intros x x' Hx y y' Hy.
+rewrite 2 spec_compare_alt; rewrite Hx, Hy; intuition.
+Qed.
+
+Add Morphism Z.lt with signature Z.eq ==> Z.eq ==> iff as NZlt_wd.
+Proof.
+intros x x' Hx y y' Hy; unfold Z.lt; rewrite Hx, Hy; intuition.
+Qed.
+
+Add Morphism Z.le with signature Z.eq ==> Z.eq ==> iff as NZle_wd.
+Proof.
+intros x x' Hx y y' Hy; unfold Z.le; rewrite Hx, Hy; intuition.
+Qed.
+
+Add Morphism Z.min with signature Z.eq ==> Z.eq ==> Z.eq as NZmin_wd.
+Proof.
+intros; red; rewrite 2 spec_min; congruence.
+Qed.
+
+Add Morphism Z.max with signature Z.eq ==> Z.eq ==> Z.eq as NZmax_wd.
+Proof.
+intros; red; rewrite 2 spec_max; congruence.
+Qed.
+
+Theorem NZlt_eq_cases : forall n m, n <= m <-> n < m \/ n == m.
+Proof.
+intros.
+unfold Z.eq; rewrite spec_lt, spec_le; omega.
+Qed.
+
+Theorem NZlt_irrefl : forall n, ~ n < n.
+Proof.
+intros; rewrite spec_lt; auto with zarith.
+Qed.
+
+Theorem NZlt_succ_r : forall n m, n < (Z.succ m) <-> n <= m.
+Proof.
+intros; rewrite spec_lt, spec_le, Z.spec_succ; omega.
+Qed.
+
+Theorem NZmin_l : forall n m, n <= m -> Z.min n m == n.
+Proof.
+intros n m; unfold Z.eq; rewrite spec_le, spec_min.
+generalize (Zmin_spec [n] [m]); omega.
+Qed.
+
+Theorem NZmin_r : forall n m, m <= n -> Z.min n m == m.
+Proof.
+intros n m; unfold Z.eq; rewrite spec_le, spec_min.
+generalize (Zmin_spec [n] [m]); omega.
+Qed.
+
+Theorem NZmax_l : forall n m, m <= n -> Z.max n m == n.
+Proof.
+intros n m; unfold Z.eq; rewrite spec_le, spec_max.
+generalize (Zmax_spec [n] [m]); omega.
+Qed.
+
+Theorem NZmax_r : forall n m, n <= m -> Z.max n m == m.
+Proof.
+intros n m; unfold Z.eq; rewrite spec_le, spec_max.
+generalize (Zmax_spec [n] [m]); omega.
+Qed.
+
+End NZOrdAxiomsMod.
+
+Definition Zopp := Z.opp.
+
+Add Morphism Z.opp with signature Z.eq ==> Z.eq as Zopp_wd.
+Proof.
+intros; zsimpl; auto with zarith.
+Qed.
+
+Theorem Zsucc_pred : forall n, Z.succ (Z.pred n) == n.
+Proof.
+red; intros; zsimpl; auto with zarith.
+Qed.
+
+Theorem Zopp_0 : - 0 == 0.
+Proof.
+red; intros; zsimpl; auto with zarith.
+Qed.
+
+Theorem Zopp_succ : forall n, - (Z.succ n) == Z.pred (- n).
+Proof.
+intros; zsimpl; auto with zarith.
+Qed.
+
+End ZSig_ZAxioms.
