theories/Numbers/Rational/BigQ/QifMake.v
@@ -24,6 +24,10 @@ Require Import QMake_base.
 
 Module Qif.
 
+ Import BinInt.
+ Open Local Scope Q_scope.
+ Open Local Scope Qc_scope.
+
  (** The notation of a rational number is either an integer x,
      interpreted as itself or a pair (x,y) of an integer x and a naturel
      number y interpreted as x/y. The pairs (x,0) and (0,y) are all
